%%%%%%%%%%%%%%%%%%%%%%%%%%%%%%%%%%%%%%%%%%%%%%%%%%%%%%%%%%%%%%%%%%%%%%%%%%%%%%%
% METADATA
%%%%%%%%%%%%%%%%%%%%%%%%%%%%%%%%%%%%%%%%%%%%%%%%%%%%%%%%%%%%%%%%%%%%%%%%%%%%%%%
\documentclass{article}
\title{Math Homework}
\author{Colbyn Wadman}

\usepackage{amsmath}
\usepackage{amssymb}

\usepackage{xurl}
\usepackage{hyperref}
\hypersetup{
    breaklinks=true,
    colorlinks=true,
}



%%%%%%%%%%%%%%%%%%%%%%%%%%%%%%%%%%%%%%%%%%%%%%%%%%%%%%%%%%%%%%%%%%%%%%%%%%%%%%%
% DOCUMENT
%%%%%%%%%%%%%%%%%%%%%%%%%%%%%%%%%%%%%%%%%%%%%%%%%%%%%%%%%%%%%%%%%%%%%%%%%%%%%%%
\begin{document}
\maketitle

 


%%%%%%%%%%%%%%%%%%%%%%%%%%%%%%%%%%%%%%%%%%%%%%%%%%%%%%%%%%%%%%%%%%%%%%%%%%%%%%%
% BODY
%%%%%%%%%%%%%%%%%%%%%%%%%%%%%%%%%%%%%%%%%%%%%%%%%%%%%%%%%%%%%%%%%%%%%%%%%%%%%%%

\section*{Problem \# 10}

\begin{equation}
\begin{split}
    \int\ln\sqrt{x} \;\mathrm{d}x
\end{split}
\end{equation}

Let

\begin{equation}
\begin{split}
    w &= \sqrt{x} \\
    \mathrm{d}w &= \frac{1}{2\sqrt{x}} \;\mathrm{d}x \\
    2\overbrace{\sqrt{x}}^{w} \;\mathrm{d}w &= \mathrm{d}x \\
    2w \;\mathrm{d}w &= \mathrm{d}x \\
\end{split}
\end{equation}

Therefore

\begin{equation}
\begin{split}
    \int\ln\sqrt{x} \;\mathrm{d}x
        &= \int\ln(w) \;\overbrace{\mathrm{d}x}^{2w \;\mathrm{d}w}
         = \int\ln(w) 2w \;\mathrm{d}w \\
        &= 2\int w \ln(w) \;\mathrm{d}w \\
\end{split}
\end{equation}

\subsection*{Subproblem}

Given

\begin{equation}
\begin{split}
    \int w \ln(w) \;\mathrm{d}w &= \int u\,\mathrm{d}v = uv - \int v \mathrm{d}u \\
\end{split}
\end{equation}

Let

\begin{equation}
    \begin{split}
        u &= \ln w \\
        \mathrm{d}u &= \frac{1}{w} \;\mathrm{d}w
    \end{split}
    \quad\leftrightarrow\quad
    \begin{split}
        v &= \frac{1}{2} w^2 \\
        \mathrm{d}v &= w \;\mathrm{d}w
    \end{split}
\end{equation}

Therefore

\begin{equation}
\begin{split}
    \int w \ln(w) \;\mathrm{d}w
        &= \left(\ln(w)\right)\left(\frac{1}{2}w^2\right) - \int\left(\frac{1}{2}w^2\right)\left(\frac{1}{w}\right)\;\mathrm{d}w \\
        &= \frac{1}{2}w^2\ln(w) - \frac{1}{2}\int\frac{w^2}{w}\;\mathrm{d}w \\
        &= \frac{1}{2}w^2\ln(w) - \frac{1}{2}\int w\;\mathrm{d}w \\
        &= \frac{1}{2}w^2\ln(w) - \frac{1}{2}\left(\frac{w^2}{2}\right) + C \\
        &= \overbrace{\frac{1}{2}w^2\ln(w) - \frac{1}{4}w^2 + C}^{w = \sqrt{x}} \\
        &= \frac{1}{2}\sqrt{x}^2\ln(\sqrt{x}) - \frac{1}{4}\sqrt{x}^2 + C \\
        &= \frac{1}{2}x\ln\sqrt{x} - \frac{1}{4}x + C \\
\end{split}
\end{equation}

\subsection*{Putting It All Together}

\begin{equation}
\begin{split}
    \int\ln\sqrt{x} \;\mathrm{d}x
        &= 2\int w \ln(w) \;\mathrm{d}w \\
        &= 2\left(\frac{1}{2}x\ln\sqrt{x} - \frac{1}{4}x\right) + C \\
        &= x\ln\sqrt{x} - \frac{1}{2}x + C
\end{split}
\end{equation}


%%%%%%%%%%%%%%%%%%%%%%%%%%%%%%%%%%%%%%%%%%%%%%%%%%%%%%%%%%%%%%%%%%%%%%%%%%%%%%%
% END
%%%%%%%%%%%%%%%%%%%%%%%%%%%%%%%%%%%%%%%%%%%%%%%%%%%%%%%%%%%%%%%%%%%%%%%%%%%%%%%
\end{document}